BridgeProperties.v
@@ -44,14 +44,14 @@ Ltac bridge_inductive_impossible_aux H:=
 Lemma preservation_bridge:
   forall Γ pc c c' m m' ev n,
     -{ Γ , pc ⊢ c }- ->
-    〈c, m 〉 ⇨+/(SL, Γ, ev, S n) 〈c', m' 〉 ->
+    〈c, m 〉 ⇨+/(SL, Γ, ev, n) 〈c', m' 〉 ->
     wf_mem m Γ ->
     (wf_mem m' Γ  /\ (c' <> STOP -> -{ Γ , pc ⊢ c' }- )) .
 
 Proof.
   intros.
   dependent induction H0.
-
+  
   - invert_low_event_step.
     forwards : preservation_event_step evt; eauto.
 
@@ -61,33 +61,32 @@ Proof.
   - invert_high_event_step.
     destruct cfg' as [c'' m''].
     forwards* (H_wf' & H_wt' ): preservation_event_step evt' c m c'' m''.
-    specializes* H_wt'.
-    replace n with (S (n - 1)) in * by omega.
-    specializes IHbridge_step_num c'' c' ___.
-Qed.    
+Qed.
 
 
 
 Lemma while_bridge_properties:
   forall Γ n e c m ev c_end m_end,
-    〈WHILE e DO c END, m 〉 ⇨+/(SL, Γ, ev, S n) 〈c_end, m_end 〉
+    〈WHILE e DO c END, m 〉 ⇨+/(SL, Γ, ev, n) 〈c_end, m_end 〉
     ->
-    n > 0 /\
-    〈 IFB e THEN c;; WHILE e DO c END ELSE SKIP FI, m〉 ⇨+/(SL, Γ, ev, n) 〈c_end, m_end 〉.
+    n >= 1 /\
+    〈 IFB e THEN c;; WHILE e DO c END ELSE SKIP FI, m〉 ⇨+/(SL, Γ, ev, n - 1) 〈c_end, m_end 〉.
 Proof.
   intros.
-  bridge_num_cases (inverts~ H) Case.
-  - Case "bridge_low_num".
-    invert_low_steps.
-  - Case "bridge_stop_num".
+  inverts~ H.
+  
+  split*.
+
+  -  exfalso. invert_low_steps.
+  - exfalso. invert_low_steps.
+  - exfalso. invert_high_steps. eauto.
+  - 
     invert_high_steps.
-    exfalso.
     invert_step.
-    auto.
-    
-  - Case "bridge_trans_num".
-    invert_high_steps.
-    invert_step; intros; subst; splits~; try omega.
+    split; try omega.
+    match goal with [ |- context [S ?x - 1]] =>
+                    replace (S x - 1 ) with x by omega
+    end; eauto.
 Qed.
 
 
@@ -96,31 +95,26 @@ Qed.
 
 Lemma if_bridge_properties:
   forall Γ n e c1 c2 m ev c_end m_end,
-    〈IFB e THEN c1 ELSE c2 FI, m 〉 ⇨+/(SL, Γ, ev, S n) 〈c_end, m_end 〉
+    〈IFB e THEN c1 ELSE c2 FI, m 〉 ⇨+/(SL, Γ, ev, n) 〈c_end, m_end 〉
     ->
-    n > 0 /\
+    n >= 1 /\
     (
-      ( exists u, (eval e m u) /\ u <> 0 /\ 〈c1, m 〉 ⇨+/(SL, Γ, ev, n) 〈c_end, m_end 〉)
+      ( exists u, (eval e m u) /\ u <> 0 /\ 〈c1, m 〉 ⇨+/(SL, Γ, ev, n - 1) 〈c_end, m_end 〉)
       \/
-      ( (eval e m 0 ) /\ 〈c2, m 〉 ⇨+/(SL, Γ, ev, n) 〈c_end, m_end 〉)
+      ( (eval e m 0 ) /\ 〈c2, m 〉 ⇨+/(SL, Γ, ev, n - 1) 〈c_end, m_end 〉)
     ).
 Proof.
   intros.
-  bridge_num_cases (inversion H) Case; subst.
-
-  - Case "bridge_low_num".
-    + invert_low_steps.
-
-  - Case "bridge_stop_num".
-    + invert_high_steps.
-      * exfalso.
-        {  - invert_step; stop_contradiction_more. }
-
-  -  Case "bridge_trans_num".
-     + invert_high_steps.
-       * invert_step; intros; subst; split; try omega.
-         { - left; exists u; split~. }
-         { - right; splits~. }
+  inverts H.
+  - exfalso. invert_low_steps.
+  - exfalso. invert_high_steps. eauto.
+  - split~ ; try omega.
+    
+    invert_high_steps.
+    invert_step; [left; exists u | right];
+    match goal with [ |- context [S ?x - 1]] =>
+                    replace (S x - 1 ) with x by omega
+    end; eauto.
 Qed.
 
 
@@ -142,31 +136,33 @@ Hint Resolve is_not_stop_trivial_exf.
 
 Lemma skip_bridge_properties:
   forall Γ n m ev c_end m_end,
-    〈SKIP, m 〉 ⇨+/(SL, Γ, ev, S n) 〈c_end, m_end 〉->
+    〈SKIP, m 〉 ⇨+/(SL, Γ, ev, n) 〈c_end, m_end 〉->
     m_end = m /\ c_end = STOP /\ n = 0 /\ ev = EmptyEvent.
 Proof.
-  intros Γ n; induction n.
-  {
-    intros.
-    invert_bridge_step_num.
-    - invert_low_steps.
-    - invert_high_steps.
-      splits~ .
-    - omega.
-  }
-  (* inductive case *)
-  {
-    
-    bridge_inductive_impossible_aux H.
-    
-  }
+  intros.
+  bridge_num_cases (inverts* H) Case.
+  - inverts H0.
+    inverts* H.
+  - inverts H0.
+    inverts H.
+    split ~ .
+  - invert_high_steps.
+    exfalso.
+    eauto.
 Qed.
 
+Ltac eval_determinism :=
+  match goal with
+    | [ H : eval ?E ?M ?V1, H' : eval ?E ?M ?V2 |- _ ] =>
+      forwards* : eval_is_det V1 V2; clear H
+  end.
 
-    
+
+
+
 Lemma assign_bridge_properties:
   forall Γ n x e m ev c_end m_end,
-    〈x ::= e, m 〉 ⇨+/(SL, Γ, ev, S n) 〈c_end, m_end 〉
+    〈x ::= e, m 〉 ⇨+/(SL, Γ, ev, n) 〈c_end, m_end 〉
     -> (exists v ℓ,
           eval e m v /\ m_end = update_st m x v
           /\ Γ (x) = Some ℓ /\
@@ -177,48 +173,51 @@ Lemma assign_bridge_properties:
        /\ (c_end = STOP)
        /\ (n = 0).
 Proof.
-  intros Γ n x e.
-  induction n; intros.
-  {
-  (*base case n = 0 *)
+  intros Γ n x e. intros.
 
-  inversion H; [ invert_low_steps | invert_high_steps | omega ]; split; auto;
-  repeat
+  inverts* H.
+  - invert_low_steps; subst.
+    split ~ .
     match goal with
-      | [ H: context [step] |- _ ] => (inverts  H;  clear H )
-      | [ H: Γ x = Some ?L, H': eval _ _ ?V |- exists _ _, _] =>
-        (exists V L)
-      | [ _ : eval ?E ?M ?V1, H' : eval ?E ?M ?V2 |- _ ] =>
-        (assert (V1 = V2) by (apply eval_is_det with (e:=E) (st:=M); crush); subst; clear H'; crush)
-      | [ H: context [AssignmentEvent ?L ?X ?V ] |- _ ] => (
-          unfold high_event in H; unfold not in H;
-          assert (low_event Γ Low (AssignmentEvent L X V))
-            by (constructor; assumption);
-          contradiction)
+        [_: context [eval e m ?v] |- _ ] =>
+        (exists v Low)
     end.
-  }
-  (* inductive case *)
-  {
-    bridge_inductive_impossible_aux H.
-  }
-Qed.
+    splits * .
+    + invert_step. eval_determinism.
+    + intros. destruct ℓ; eauto; impossible_flows.
+    + intros.  destruct ℓ; eauto; impossible_flows.
+    + intros. exfalso. eauto.
+  - invert_high_steps; subst.
+    splits ~ .
+    match goal with
+        [_: context [eval e m ?v], _:  Γ _ = Some ?ℓ |- _ ] =>
+        (exists v ℓ)
+    end.
+
+    splits ~ .
+    + invert_step. eval_determinism.
+    + intros. exfalso. eauto.
+  - exfalso.
+    invert_high_steps.
+    eauto.
+Qed.  
 
 
 
 Lemma seq_comp_bridge_property:
   forall Γ n c1 c2 m ev c_end m_end,
-    〈c1;; c2, m 〉 ⇨+/(SL, Γ, ev, S n) 〈c_end, m_end 〉
+    〈c1;; c2, m 〉 ⇨+/(SL, Γ, ev, n) 〈c_end, m_end 〉
     ->
-    (exists c1', 〈c1, m 〉 ⇨+/(SL, Γ, ev, S n) 〈 c1', m_end 〉
+    (exists c1', 〈c1, m 〉 ⇨+/(SL, Γ, ev, n) 〈 c1', m_end 〉
                  /\ (c1' <> STOP -> c_end = (c1';; c2))
                  /\ (c1' = STOP -> c_end = c2)
                  /\ low_event Γ Low ev
     )
     \/
     (exists m1' k,
-        k < n /\ n  > 0 /\
-       〈c1, m 〉 ⇨+/(SL, Γ, EmptyEvent, S k) 〈 STOP, m1' 〉
-       /\ 〈c2, m1' 〉 ⇨+/(SL, Γ, ev, n - k ) 〈 c_end, m_end 〉
+        k < n /\ n > 0 /\
+       〈c1, m 〉 ⇨+/(SL, Γ, EmptyEvent, k) 〈 STOP, m1' 〉
+       /\ 〈c2, m1' 〉 ⇨+/(SL, Γ, ev, n - k - 1 ) 〈 c_end, m_end 〉
     ).
 Proof.
   intros Γ n.
@@ -226,26 +225,25 @@ Proof.
   (* base case *)
   {
     left.
-   intros.
-   bridge_num_cases (inversion H) Case; subst.
-   Case "bridge_low_num".
-   {
-     do 2
-        match goal with
+    intros.
+
+    inverts* H.
+    (* 2 cases *)
+    - (* low-step*)
+      do 2
+      match goal with
           | [ H : context [low_event_step] |- _ ] =>
-            (inversion H ; subst; clear H)
+            (inverts H ; clear H)
           | [ H : context [event_step _ _ 〈 c1;; c2, _ 〉 _] |- _ ] =>
-            (inversion H ; subst; clear H);
+            (inverts H ; clear H);
               match goal with
-                | [ H : context [event_step _ _ 〈c1, _ 〉〈?C1, _ 〉] |- _ ] =>
-                  (exists C1; repeat ( constructor || assumption))
-              end
-        end;
-     match goal with | [ H :  context [low_event] |- _ ] => inversion H end;
-     crush.
-   }
-   Case "bridge_stop_num".
-   {
+                  | [ H : context [event_step _ _ 〈c1, _ 〉〈?C1, _ 〉] |- _ ] =>
+                    (exists C1; repeat ( constructor || assumption))
+                end;
+              intros;         exfalso;eauto
+
+        end.
+    - (* high_step *)
      
      repeat
        match goal with
@@ -261,17 +259,13 @@ Proof.
          | [ H : context [ _ = 〈 STOP, _ 〉] |- _ ] =>
            inversion H; clear H; contradiction
        end.
-   }
-   Case "bridge_trans_num".
-   {
-     omega.
-   }
   }
   (* inductive case *)
   {
     intros.
-    inversion H.
-    subst.
+    inverts H.
+
+    
 
     do 3
        match goal with
@@ -282,16 +276,18 @@ Proof.
            inversion H; subst; clear H
 
        end.
+    
+
     {
 
       match goal with
-        | [ H: 〈?c1';; c2, ?st' 〉 ⇨+/(SL, Γ, ev, S n) 〈c_end, m_end 〉 |- _ ]
+        | [ H: 〈?c1';; c2, ?st' 〉 ⇨+/(SL, Γ, ev, n) 〈c_end, m_end 〉 |- _ ]
           => specialize (IHn c1' c2 st' ev c_end m_end H)
       end.
       destruct IHn.
       {
         super_destruct.
-        match goal with [ H:〈c1', st' 〉 ⇨+/(SL, Γ, ev, S n) 〈?x, m_end 〉 |- _ ] =>
+        match goal with [ H:〈c1', st' 〉 ⇨+/(SL, Γ, ev,  n) 〈?x, m_end 〉 |- _ ] =>
                         rename x into c1_end
         end.
         left.
@@ -302,12 +298,12 @@ Proof.
       }
       {
         super_destruct.
-        match goal with [ H:〈c2, ?X 〉 ⇨+/(SL, Γ, ev, n - ?K ) 〈c_end, m_end 〉|- _ ] =>
+        match goal with [ H:〈c2, ?X 〉 ⇨+/(SL, Γ, ev, n - ?K -1 ) 〈c_end, m_end 〉|- _ ] =>
                         rename X into m1_end;
                           rename K into k
         end.
         right; exists m1_end (S k).
-        repeat (split || auto || omega).
+        splits*; try omega.
         apply bridge_trans_num with evt' 〈c1', st' 〉; eauto.
       }
     }
@@ -322,7 +318,7 @@ Proof.
       apply bridge_stop_num with evt'; eauto.
       
       unfolds is_not_stop;
-      assert (( S n) - 0 = S n ) as X  by omega.
+      assert (( S n - 0 - 1 =  n )) as X  by omega.
       rewrite X.
       assumption.
     }
